src/lang1.v
@@ -13,16 +13,34 @@ Variant head_step {n : nat} : comp n -> unit -> list unit -> comp n -> unit -> l
 | cstep_step c1 c2 : cstep c1 c2 ->
                      head_step c1 tt nil c2 tt nil.
 
+
+Lemma Inj_fill n:
+  ∀ Ki : ectx, Inj eq eq (@fill n Ki).
+Proof.
+  intros. induction Ki; repeat intro; auto; inv H; apply IHKi; auto.
+Qed.
+
+Lemma to_of_val n v : to_val n (of_val n v) = Some v.
+  Proof. by induction v; simplify_option_eq. Qed.
+
+
 Lemma lang_mixin n : EctxiLanguageMixin (of_val n) (to_val n) fill head_step.
 Proof.
   split; auto.
   - unfold of_val, to_val. intros. destruct e; inversion H; auto.
   - intros. inversion H. subst. inversion H0. subst. inv H1; destruct C; simpl; auto.
   - intros. destruct Ki; simpl in *; auto; try inv H; inv H0.
-  - intros. induction Ki; repeat intro; auto; inv H; apply IHKi; auto.
-  - intros.
-    destruct Ki1, Ki2; inv H1; auto. simpl in H2.
-    inv H2.
+  - apply Inj_fill.
+  - induction Ki1, Ki2; intros; try discriminate; simplify_eq;
+    repeat match goal with
+           | H : to_val (of_val _) = None |- _ => by rewrite to_of_val in H
+           end; auto.
+    eapply IHKi1 in H1; subst; eauto.
+    eapply IHKi1 in H2; subst; eauto.
+    eapply IHKi1 in H1; subst; eauto.
+  - destruct Ki; inversion_clear 1; simplify_option_eq; eauto.
+    inv H0. 
+    inv H0. 
   split; apply _ || eauto using to_of_val, of_to_val, val_head_stuck,
          fill_item_.,`val, fill_item_no_val_inj, head_ctx_step_val.
 Qed.
